Runtime/Network/Execution/Next.lean
@@ -2,7 +2,7 @@ import Runtime.Network.Execution.Basic
 
 namespace Network.Executable    
 
-private def nextTime (exec : Executable net) : Option (Time.From exec.tag.time) :=
+def nextTime (exec : Executable net) : Option (Time.From exec.time) :=
   match h : exec.queue[0]? with 
   | none => none
   | some nextEvent => some ⟨nextEvent.time, exec.lawfulQueue h⟩
@@ -20,11 +20,11 @@ private def eventSplit (exec : Executable net) (time : Time) : Array (Event net)
   let ⟨next, postponed⟩ := candidates.unique (·.id)
   (next, postponed ++ later)
 
-theorem eventSplit_fst_LawfulQueue {exec : Executable net} : 
+theorem eventSplit_fst_LawfulQueue {exec : Executable net} {time} : 
   LawfulQueue (exec.eventSplit time).fst time := sorry
   -- TODO: We need theorems about `Array.unique/.split` to prove this.
 
-theorem eventSplit_snd_LawfulQueue {exec : Executable net} : 
+theorem eventSplit_snd_LawfulQueue {exec : Executable net} {time} : 
   LawfulQueue (exec.eventSplit time).snd time := sorry
   -- TODO: We need theorems about `Array.unique/.split` to prove this.
 
@@ -44,45 +44,42 @@ structure Next (net : Network) where
   queue       : Array (Event net)
   lawfulQueue : LawfulQueue queue tag.time
 
-protected def Next.for (exec : Executable net) : Option (Next net) := 
-  match exec.nextTime with 
-  | none => none
-  | some time =>
-    let tag := exec.tag.advance time
-    let eventSplit := exec.eventSplit time -- TODO: We can't destruct here, as this causes problems in the proof of `lawfulQueue`.
-    let events := eventSplit.fst
-    let later := eventSplit.snd
-    let timers := events.filterMap (·.timer?)
-    let timerEvents := exec.nextTimerEvents timers time
-    let queue := later.merge timerEvents
-    some { tag, events, queue, lawfulQueue := (exec.tag.advance_time time) ▸ LawfulQueue.merge eventSplit_snd_LawfulQueue nextTimerEvents_LawfulQueue }
+namespace Next
 
-theorem Next.for_isSome_iff_nextTime_isSome {exec : Executable net} :
-  (Next.for exec).isSome ↔ exec.nextTime.isSome := by
-  simp [Next.for]
-  constructor <;> split <;> simp_all [Option.isSome]
-    
-theorem Next.for_isSome_iff_queue_not_isEmpty {exec : Executable net} :
-  (Next.for exec).isSome ↔ ¬exec.queue.isEmpty := by
-  simp [for_isSome_iff_nextTime_isSome, nextTime_isSome_iff_queue_not_isEmpty]
+def empty (tag : Tag) : Next net where
+  tag := tag
+  events := #[]
+  queue := #[]
+  lawfulQueue := LawfulQueue.empty
 
-theorem Next.for_preserves_events : (Next.for exec = some next) → ∃ timerEvents, (next.events ++ next.queue) ~ (exec.queue ++ timerEvents) := by
+protected def «for» (exec : Executable net) (time : Time.From exec.time) : Next net := 
+  let eventSplit := exec.eventSplit time -- TODO: We can't destruct here, as this causes problems in the proof of `lawfulQueue`.
+  let events := eventSplit.fst
+  let later := eventSplit.snd
+  let timers := events.filterMap (·.timer?)
+  let timerEvents := exec.nextTimerEvents timers time
+  { 
+    tag         := exec.tag.advance time
+    queue       := later.merge timerEvents
+    lawfulQueue := (exec.tag.advance_time time) ▸ LawfulQueue.merge eventSplit_snd_LawfulQueue nextTimerEvents_LawfulQueue 
+    events
+  }
+
+theorem for_preserves_events {time} : (Next.for exec time = next) → ∃ timerEvents, (next.events ++ next.queue) ~ (exec.queue ++ timerEvents) := by
   intro h
   simp [Next.for] at h
-  split at h
-  · contradiction
-  case _ time _ =>
-    simp at h
-    let events := (exec.eventSplit time).fst
-    let timers := events.filterMap (·.timer?)
-    exists exec.nextTimerEvents timers time
-    sorry 
+  let events := (exec.eventSplit time).fst
+  let timers := events.filterMap (·.timer?)
+  exists exec.nextTimerEvents timers time
+  sorry 
 
 -- The actions-interface for a given reactor according to the `Next` instance.
-def Next.actions (next : Next net) (reactor : ReactorId net) : Interface? (reactor.class.interface .actions) := 
+def actions (next : Next net) (reactor : ReactorId net) : Interface? (reactor.class.interface .actions) := 
   fun action => 
     match h : next.events.findP? (·.id = .action ⟨reactor, action⟩) with
     | none => none
     | some event => have h := Array.findP?_property h; event.actionValue (of_decide_eq_true h)
+
+end Next
 
 end Network.Executable
